\documentclass[a4paper,landscape]{jarticle}
\usepackage{proof}
\begin{document}
\[
\infer[\texttt{(\_ th-lemma arith farkas 3/2 1/2 1/2 1)}]{\mbox{\texttt{false}}}{\infer[\texttt{unit-resolution}]{\mbox{\texttt{(<= x3 0.0)}}}{\infer[\texttt{mp}]{\mbox{\texttt{(or (not c4) (<= x3 0.0))}}}{\infer[\texttt{asserted}]{\mbox{\texttt{(=> c4 (>= (- x3) 0.0))}}}{} & \infer[\texttt{trans}]{\mbox{\texttt{(= (=> c4 (>= (- x3) 0.0)) (or (not c4) (<= x3 0.0)))}}}{\infer[\texttt{trans}]{\mbox{\texttt{(= (=> c4 (>= (- x3) 0.0)) (or (not c4) (>= ($*$ (- 1.0) x3) 0.0)))}}}{\infer[\texttt{monotonicity}]{\mbox{\texttt{(= (=> c4 (>= (- x3) 0.0)) (=> c4 (>= ($*$ (- 1.0) x3) 0.0)))}}}{\infer[\texttt{monotonicity}]{\mbox{\texttt{(= (>= (- x3) 0.0) (>= ($*$ (- 1.0) x3) 0.0))}}}{\infer[\texttt{rewrite}]{\mbox{\texttt{(= (- x3) ($*$ (- 1.0) x3))}}}{}}} & \infer[\texttt{rewrite}]{\mbox{\texttt{(= (=> c4 (>= ($*$ (- 1.0) x3) 0.0)) (or (not c4) (>= ($*$ (- 1.0) x3) 0.0)))}}}{}} & \infer[\texttt{monotonicity}]{\mbox{\texttt{(= (or (not c4) (>= ($*$ (- 1.0) x3) 0.0)) (or (not c4) (<= x3 0.0)))}}}{\infer[\texttt{rewrite}]{\mbox{\texttt{(= (>= ($*$ (- 1.0) x3) 0.0) (<= x3 0.0))}}}{}}}} & \infer[\texttt{asserted}]{\mbox{\texttt{c4}}}{}} & \infer[\texttt{unit-resolution}]{\mbox{\texttt{(<= (+ x1 ($*$ (- 1.0) x2)) 0.0)}}}{\infer[\texttt{mp}]{\mbox{\texttt{(or (not c2) (<= (+ x1 ($*$ (- 1.0) x2)) 0.0))}}}{\infer[\texttt{asserted}]{\mbox{\texttt{(=> c2 (>= (+ (- x1) x2) 0.0))}}}{} & \infer[\texttt{trans}]{\mbox{\texttt{(= (=> c2 (>= (+ (- x1) x2) 0.0)) (or (not c2) (<= (+ x1 ($*$ (- 1.0) x2)) 0.0)))}}}{\infer[\texttt{trans}]{\mbox{\texttt{(= (=> c2 (>= (+ (- x1) x2) 0.0)) (or (not c2) (>= (+ ($*$ (- 1.0) x1) x2) 0.0)))}}}{\infer[\texttt{monotonicity}]{\mbox{\texttt{(= (=> c2 (>= (+ (- x1) x2) 0.0)) (=> c2 (>= (+ ($*$ (- 1.0) x1) x2) 0.0)))}}}{\infer[\texttt{monotonicity}]{\mbox{\texttt{(= (>= (+ (- x1) x2) 0.0) (>= (+ ($*$ (- 1.0) x1) x2) 0.0))}}}{\infer[\texttt{monotonicity}]{\mbox{\texttt{(= (+ (- x1) x2) (+ ($*$ (- 1.0) x1) x2))}}}{\infer[\texttt{rewrite}]{\mbox{\texttt{(= (- x1) ($*$ (- 1.0) x1))}}}{}}}} & \infer[\texttt{rewrite}]{\mbox{\texttt{(= (=> c2 (>= (+ ($*$ (- 1.0) x1) x2) 0.0)) (or (not c2) (>= (+ ($*$ (- 1.0) x1) x2) 0.0)))}}}{}} & \infer[\texttt{monotonicity}]{\mbox{\texttt{(= (or (not c2) (>= (+ ($*$ (- 1.0) x1) x2) 0.0)) (or (not c2) (<= (+ x1 ($*$ (- 1.0) x2)) 0.0)))}}}{\infer[\texttt{rewrite}]{\mbox{\texttt{(= (>= (+ ($*$ (- 1.0) x1) x2) 0.0) (<= (+ x1 ($*$ (- 1.0) x2)) 0.0))}}}{}}}} & \infer[\texttt{asserted}]{\mbox{\texttt{c2}}}{}} & \infer[\texttt{unit-resolution}]{\mbox{\texttt{(>= (+ x1 x2 x3) 1.0)}}}{\infer[\texttt{mp}]{\mbox{\texttt{(or (not c1) (>= (+ x1 x2 x3) 1.0))}}}{\infer[\texttt{asserted}]{\mbox{\texttt{(=> c1 (>= (+ x1 x2 x3) 1.0))}}}{} & \infer[\texttt{rewrite}]{\mbox{\texttt{(= (=> c1 (>= (+ x1 x2 x3) 1.0)) (or (not c1) (>= (+ x1 x2 x3) 1.0)))}}}{}} & \infer[\texttt{asserted}]{\mbox{\texttt{c1}}}{}} & \infer[\texttt{unit-resolution}]{\mbox{\texttt{(<= (+ x2 ($*$ (- 1.0) x3)) 0.0)}}}{\infer[\texttt{mp}]{\mbox{\texttt{(or (not c3) (<= (+ x2 ($*$ (- 1.0) x3)) 0.0))}}}{\infer[\texttt{asserted}]{\mbox{\texttt{(=> c3 (>= (+ (- x2) x3) 0.0))}}}{} & \infer[\texttt{trans}]{\mbox{\texttt{(= (=> c3 (>= (+ (- x2) x3) 0.0)) (or (not c3) (<= (+ x2 ($*$ (- 1.0) x3)) 0.0)))}}}{\infer[\texttt{trans}]{\mbox{\texttt{(= (=> c3 (>= (+ (- x2) x3) 0.0)) (or (not c3) (>= (+ ($*$ (- 1.0) x2) x3) 0.0)))}}}{\infer[\texttt{monotonicity}]{\mbox{\texttt{(= (=> c3 (>= (+ (- x2) x3) 0.0)) (=> c3 (>= (+ ($*$ (- 1.0) x2) x3) 0.0)))}}}{\infer[\texttt{monotonicity}]{\mbox{\texttt{(= (>= (+ (- x2) x3) 0.0) (>= (+ ($*$ (- 1.0) x2) x3) 0.0))}}}{\infer[\texttt{monotonicity}]{\mbox{\texttt{(= (+ (- x2) x3) (+ ($*$ (- 1.0) x2) x3))}}}{\infer[\texttt{rewrite}]{\mbox{\texttt{(= (- x2) ($*$ (- 1.0) x2))}}}{}}}} & \infer[\texttt{rewrite}]{\mbox{\texttt{(= (=> c3 (>= (+ ($*$ (- 1.0) x2) x3) 0.0)) (or (not c3) (>= (+ ($*$ (- 1.0) x2) x3) 0.0)))}}}{}} & \infer[\texttt{monotonicity}]{\mbox{\texttt{(= (or (not c3) (>= (+ ($*$ (- 1.0) x2) x3) 0.0)) (or (not c3) (<= (+ x2 ($*$ (- 1.0) x3)) 0.0)))}}}{\infer[\texttt{rewrite}]{\mbox{\texttt{(= (>= (+ ($*$ (- 1.0) x2) x3) 0.0) (<= (+ x2 ($*$ (- 1.0) x3)) 0.0))}}}{}}}} & \infer[\texttt{asserted}]{\mbox{\texttt{c3}}}{}}}
\]
\end{document}
