\documentclass[a4paper,landscape]{jarticle}
\usepackage{proof}
\begin{document}
\[
\infer[\texttt{(\_ th-lemma arith farkas 3/2 1/2 1/2 1)}]{\mbox{\texttt{false}}}{
  \infer[\texttt{mp}]{\mbox{\texttt{(<= x3 0.0)}}}{
    \infer[\texttt{asserted}]{\mbox{\texttt{(>= (- x3) 0.0)}}}{}
    &
    \infer[\texttt{trans}]{\mbox{\texttt{(= (>= (- x3) 0.0) (<= x3 0.0))}}}{
      \infer[\texttt{monotonicity}]{\mbox{\texttt{(= (>= (- x3) 0.0) (>= ($*$ (- 1.0) x3) 0.0))}}}{
        \infer[\texttt{rewrite}]{\mbox{\texttt{(= (- x3) ($*$ (- 1.0) x3))}}}{}
      }
      &
      \infer[\texttt{rewrite}]{\mbox{\texttt{(= (>= ($*$ (- 1.0) x3) 0.0) (<= x3 0.0))}}}{}
    }
  }
  &
  \infer[\texttt{mp}]{\mbox{\texttt{(<= (+ x1 ($*$ (- 1.0) x2)) 0.0)}}}{
    \infer[\texttt{asserted}]{\mbox{\texttt{(>= (+ (- x1) x2) 0.0)}}}{}
    &
    \infer[\texttt{trans}]{\mbox{\texttt{(= (>= (+ (- x1) x2) 0.0) (<= (+ x1 ($*$ (- 1.0) x2)) 0.0))}}}{
      \infer[\texttt{monotonicity}]{\mbox{\texttt{(= (>= (+ (- x1) x2) 0.0) (>= (+ ($*$ (- 1.0) x1) x2) 0.0))}}}{
        \infer[\texttt{monotonicity}]{\mbox{\texttt{(= (+ (- x1) x2) (+ ($*$ (- 1.0) x1) x2))}}}{
          \infer[\texttt{rewrite}]{\mbox{\texttt{(= (- x1) ($*$ (- 1.0) x1))}}}{}
        }
      }
      &
      \infer[\texttt{rewrite}]{\mbox{\texttt{(= (>= (+ ($*$ (- 1.0) x1) x2) 0.0) (<= (+ x1 ($*$ (- 1.0) x2)) 0.0))}}}{}
    }
  }
  &
  \infer[\texttt{asserted}]{\mbox{\texttt{(>= (+ x1 x2 x3) 1.0)}}}{}
  &
  \infer[\texttt{mp}]{\mbox{\texttt{(<= (+ x2 ($*$ (- 1.0) x3)) 0.0)}}}{
    \infer[\texttt{asserted}]{\mbox{\texttt{(>= (+ (- x2) x3) 0.0)}}}{}
    &
    \infer[\texttt{trans}]{\mbox{\texttt{(= (>= (+ (- x2) x3) 0.0) (<= (+ x2 ($*$ (- 1.0) x3)) 0.0))}}}{
      \infer[\texttt{monotonicity}]{\mbox{\texttt{(= (>= (+ (- x2) x3) 0.0) (>= (+ ($*$ (- 1.0) x2) x3) 0.0))}}}{
        \infer[\texttt{monotonicity}]{\mbox{\texttt{(= (+ (- x2) x3) (+ ($*$ (- 1.0) x2) x3))}}}{
          \infer[\texttt{rewrite}]{\mbox{\texttt{(= (- x2) ($*$ (- 1.0) x2))}}}{}
        }
      }
      &
      \infer[\texttt{rewrite}]{\mbox{\texttt{(= (>= (+ ($*$ (- 1.0) x2) x3) 0.0) (<= (+ x2 ($*$ (- 1.0) x3)) 0.0))}}}{}
    }
  }
}
\]
\end{document}
